AwsCryptographicMaterialProviders/dafny/AwsCryptographyKeyStore/src/DefaultKeyStorageInterface.dfy
@@ -3,6 +3,8 @@
 include "../Model/AwsCryptographyKeyStoreTypes.dfy"
 include "Structure.dfy"
 include "ErrorMessages.dfy"
+include "KmsArn.dfy"
+include "StorageHelpers.dfy"
 
 module DefaultKeyStorageInterface {
   import opened Wrappers
@@ -12,9 +14,17 @@ module DefaultKeyStorageInterface {
   import DDB = ComAmazonawsDynamodbTypes
   import UTF8
   import Structure
+  import String = StandardLibrary.String
+  import KmsArn
+  import StorageHelpers
 
-  const ToAttributeMap := Structure.ToAttributeMap
-  const ToEncryptedHierarchicalKey := Structure.ToEncryptedHierarchicalKey
+  const ToAttributeMap := StorageHelpers.ToAttributeMap
+  const ToEncryptedHierarchicalKey := StorageHelpers.ToEncryptedHierarchicalKey
+  const MutationCommitmentFromOptionalItem := StorageHelpers.MutationCommitmentFromOptionalItem
+  const MutationIndexFromOptionalItem := StorageHelpers.MutationIndexFromOptionalItem
+  const EncryptedHierarchicalKeyFromItem := StorageHelpers.EncryptedHierarchicalKeyFromItem
+  const BlobToExclusiveStartKey := StorageHelpers.BlobToExclusiveStartKey
+  const LastEvaluatedKeyToBlob := StorageHelpers.LastEvaluatedKeyToBlob
   import ErrorMessages = KeyStoreErrorMessages
 
   const BRANCH_KEY_EXISTS_EXPRESSION_ATTRIBUTE_NAME := "#BranchKeyIdentifierField"
@@ -24,10 +34,30 @@ module DefaultKeyStorageInterface {
        ]
   const BRANCH_KEY_NOT_EXIST_CONDITION := "attribute_not_exists(" + BRANCH_KEY_EXISTS_EXPRESSION_ATTRIBUTE_NAME + ")"
   const BRANCH_KEY_EXISTS_CONDITION := "attribute_exists(" + BRANCH_KEY_EXISTS_EXPRESSION_ATTRIBUTE_NAME + ")"
+  // The Table's Index is BRANCH_KEY_IDENTIFIER_FIELD & TYPE_FIELD
+  const INDEX_EXP_ATT_NAMES: DDB.ExpressionAttributeNameMap :=
+    map[
+      "#pk" := Structure.BRANCH_KEY_IDENTIFIER_FIELD,
+      "#sk" := Structure.TYPE_FIELD]
+  // Ideally, MAX_PAGE would be Types.UInt.uint8, but the size of sequence is always an int
+  const DDB_MAX_MUTATION_WRITE_PAGE_SIZE: int := 98
+  const DDB_MAX_MUTATION_WRITE_PAGE_SIZE_str: string := "98"
 
   datatype ConditionExpression =
     | BRANCH_KEY_NOT_EXIST
     | BRANCH_KEY_EXISTS
+
+  // To use these values in a match Dafny needs to match these as local variables.
+  // This means that Dafny can not use `Structure.MUTATION_COMMITMENT_TYPE`
+  // in the case statement to evaluate a literal.
+  const MUTATION_COMMITMENT_TYPE := "branch:MUTATION_COMMITMENT" // Structure.MUTATION_COMMITMENT_TYPE
+  const MUTATION_INDEX_TYPE := "branch:MUTATION_INDEX" // Structure.MUTATION_INDEX_TYPE
+
+  lemma TypesAreCorrect()
+    ensures
+      && MUTATION_COMMITMENT_TYPE == Structure.MUTATION_COMMITMENT_TYPE
+      && MUTATION_INDEX_TYPE == Structure.MUTATION_INDEX_TYPE
+  {}
 
   class {:termination false} DynamoDBKeyStorageInterface
     //= aws-encryption-sdk-specification/framework/key-store/dynamodb-key-storage.md#operations
@@ -60,6 +90,30 @@ module DefaultKeyStorageInterface {
       output: Result<Types.WriteNewEncryptedBranchKeyOutput, Types.Error>
     )
     {true}
+
+    predicate WriteMutationIndexEnsuresPublicly(
+      input: Types.WriteMutationIndexInput,
+      output: Result<Types.WriteMutationIndexOutput, Types.Error>
+    )
+    {true}
+
+    predicate GetMutationEnsuresPublicly(
+      input: Types.GetMutationInput,
+      output: Result<Types.GetMutationOutput, Types.Error>
+    )
+    {
+      && (output.Success? ==>
+            // Conditions for M-Lock
+            && (output.value.MutationCommitment.Some? ==>
+                  && output.value.MutationCommitment.value.Identifier == input.Identifier
+                  && Structure.MutationCommitment?(output.value.MutationCommitment.value))
+               // Conditions for M-Index
+            && (output.value.MutationIndex.Some? ==>
+                  && output.value.MutationIndex.value.Identifier == input.Identifier
+                  && Structure.MutationIndex?(output.value.MutationIndex.value) )
+      )
+    }
+
     predicate WriteNewEncryptedBranchKeyVersionEnsuresPublicly(
       input: Types.WriteNewEncryptedBranchKeyVersionInput ,
       output: Result<Types.WriteNewEncryptedBranchKeyVersionOutput, Types.Error>
@@ -113,9 +167,14 @@ module DefaultKeyStorageInterface {
                //# to items retrieved from the table.
             && output.value.Item.EncryptionContext[Structure.TABLE_FIELD] == logicalKeyStoreName
       )
-
-
     }
+
+    predicate WriteAtomicMutationEnsuresPublicly(
+      input: Types.WriteAtomicMutationInput,
+      output: Result<Types.WriteAtomicMutationOutput, Types.Error>
+    )
+    {true}
+
     predicate GetEncryptedBeaconKeyEnsuresPublicly(
       input: Types.GetEncryptedBeaconKeyInput ,
       output: Result<Types.GetEncryptedBeaconKeyOutput, Types.Error>
@@ -137,9 +196,70 @@ module DefaultKeyStorageInterface {
             && output.value.Item.EncryptionContext[Structure.TABLE_FIELD] == logicalKeyStoreName
       )
     }
+
+    predicate DeleteMutationEnsuresPublicly(
+      input: Types.DeleteMutationInput,
+      output: Result<Types.DeleteMutationOutput, Types.Error>
+    )
+    {true}
+
     predicate GetKeyStorageInfoEnsuresPublicly(
       input: Types.GetKeyStorageInfoInput ,
       output: Result<Types.GetKeyStorageInfoOutput, Types.Error>
+    )
+    {true}
+
+    predicate GetItemsForInitializeMutationEnsuresPublicly(
+      input: Types.GetItemsForInitializeMutationInput ,
+      output: Result<Types.GetItemsForInitializeMutationOutput, Types.Error>
+    )
+    {
+      && (output.Success? ==>
+            // Conditions for Active
+            && output.value.ActiveItem.Identifier == input.Identifier
+            && Structure.ActiveHierarchicalSymmetricKey?(output.value.ActiveItem)
+            && output.value.ActiveItem.EncryptionContext[Structure.TABLE_FIELD] == logicalKeyStoreName
+            && KmsArn.ValidKmsArn?(output.value.ActiveItem.KmsArn)
+               // Conditions for Beacon
+            && output.value.BeaconItem.Identifier == input.Identifier
+            && Structure.ActiveHierarchicalSymmetricBeaconKey?(output.value.BeaconItem)
+            && output.value.BeaconItem.EncryptionContext[Structure.TABLE_FIELD] == logicalKeyStoreName
+            && KmsArn.ValidKmsArn?(output.value.BeaconItem.KmsArn)
+               // Conditions for M-Lock
+            && (output.value.MutationCommitment.Some? ==>
+                  && output.value.MutationCommitment.value.Identifier == input.Identifier
+                  && Structure.MutationCommitment?(output.value.MutationCommitment.value))
+               // Conditions for M-Index
+            && (output.value.MutationIndex.Some? ==>
+                  && output.value.MutationIndex.value.Identifier == input.Identifier
+                  && Structure.MutationIndex?(output.value.MutationIndex.value) )
+      )
+    }
+
+    predicate WriteInitializeMutationEnsuresPublicly(
+      input: Types.WriteInitializeMutationInput ,
+      output: Result<Types.WriteInitializeMutationOutput, Types.Error>
+    )
+    {true}
+
+    predicate QueryForVersionsEnsuresPublicly(
+      input: Types.QueryForVersionsInput ,
+      output: Result<Types.QueryForVersionsOutput, Types.Error>
+    )
+    {
+      && (output.Success? && |output.value.Items| > 0 ==>
+            forall item <- output.value.Items ::
+              && item.Identifier == input.Identifier
+              && Structure.DecryptOnlyHierarchicalSymmetricKey?(item)
+              && item.Type.HierarchicalSymmetricVersion?
+              && item.EncryptionContext[Structure.TABLE_FIELD] == logicalKeyStoreName
+              && KmsArn.ValidKmsArn?(item.KmsArn)
+      )
+    }
+
+    predicate WriteMutatedVersionsEnsuresPublicly(
+      input: Types.WriteMutatedVersionsInput ,
+      output: Result<Types.WriteMutatedVersionsOutput, Types.Error>
     )
     {true}
 
@@ -226,10 +346,9 @@ module DefaultKeyStorageInterface {
                     //#  - Item: A [record formatted item](#record-format) constructed from the version input
                     //#  - ConditionExpression: `attribute_not_exists(branch-key-id)`
                     //#  - TableName: the configured Table Name
-                    CreateTransactWritePutItem(
+                    TransactCreateHKey(
                       input.Version,
-                      ddbTableName,
-                      BRANCH_KEY_NOT_EXIST
+                      ddbTableName
                     ),
                     //= aws-encryption-sdk-specification/framework/key-store/dynamodb-key-storage.md#writenewencryptedbranchkey
                     //= type=implication
@@ -237,10 +356,9 @@ module DefaultKeyStorageInterface {
                     //#  - Item: A [record formatted item](#record-format) constructed from the active input
                     //#  - ConditionExpression: `attribute_not_exists(branch-key-id)`
                     //#  - TableName: the configured Table Name
-                    CreateTransactWritePutItem(
+                    TransactCreateHKey(
                       input.Active,
-                      ddbTableName,
-                      BRANCH_KEY_NOT_EXIST
+                      ddbTableName
                     ),
                     //= aws-encryption-sdk-specification/framework/key-store/dynamodb-key-storage.md#writenewencryptedbranchkey
                     //= type=implication
@@ -248,10 +366,9 @@ module DefaultKeyStorageInterface {
                     //#  - Item: A [record formatted item](#record-format) constructed from the beacon input
                     //#  - ConditionExpression: `attribute_not_exists(branch-key-id)`
                     //#  - TableName is the configured Table Name
-                    CreateTransactWritePutItem(
+                    TransactCreateHKey(
                       input.Beacon,
-                      ddbTableName,
-                      BRANCH_KEY_NOT_EXIST
+                      ddbTableName
                     )
                   ]
                 )
@@ -285,28 +402,22 @@ module DefaultKeyStorageInterface {
       );
 
       var items: DDB.TransactWriteItemList := [
-        CreateTransactWritePutItem(
+        TransactCreateHKey(
           input.Version,
-          ddbTableName,
-          BRANCH_KEY_NOT_EXIST
+          ddbTableName
         ),
-        CreateTransactWritePutItem(
+        TransactCreateHKey(
           input.Active,
-          ddbTableName,
-          BRANCH_KEY_NOT_EXIST
+          ddbTableName
         ),
-        CreateTransactWritePutItem(
+        TransactCreateHKey(
           input.Beacon,
-          ddbTableName,
-          BRANCH_KEY_NOT_EXIST
+          ddbTableName
         )
       ];
 
       var transactRequest := DDB.TransactWriteItemsInput(
-        TransactItems := items,
-        ReturnConsumedCapacity := None,
-        ReturnItemCollectionMetrics := None,
-        ClientRequestToken := None
+        TransactItems := items
       );
 
       var transactWriteItemsResponse? := ddbClient.TransactWriteItems(transactRequest);
@@ -333,7 +444,7 @@ module DefaultKeyStorageInterface {
       //# The call to Amazon DynamoDB TransactWriteItems MUST use the configured Amazon DynamoDB Client to make the call.
       ensures
         && (forall k <- input.Version.EncryptionContext.Keys :: DDB.IsValid_AttributeName(k))
-        && (forall k <- input.Active.EncryptionContext.Keys :: DDB.IsValid_AttributeName(k))
+        && (forall k <- input.Active.Item.EncryptionContext.Keys :: DDB.IsValid_AttributeName(k))
         ==>
           && |ddbClient.History.TransactWriteItems| == |old(ddbClient.History.TransactWriteItems)| + 1
           && old(ddbClient.History.TransactWriteItems) < ddbClient.History.TransactWriteItems
@@ -344,7 +455,7 @@ module DefaultKeyStorageInterface {
         output.Success?
         ==>
           && (forall k <- input.Version.EncryptionContext.Keys :: DDB.IsValid_AttributeName(k))
-          && (forall k <- input.Active.EncryptionContext.Keys :: DDB.IsValid_AttributeName(k))
+          && (forall k <- input.Active.Item.EncryptionContext.Keys :: DDB.IsValid_AttributeName(k))
              //= aws-encryption-sdk-specification/framework/key-store/dynamodb-key-storage.md#writenewencryptedbranchkeyversion
              //= type=implication
              //# To add the new branch key to the keystore,
@@ -361,10 +472,9 @@ module DefaultKeyStorageInterface {
                     //#  - Item: A [record formatted item](#record-format) constructed from the version input
                     //#  - ConditionExpression: `attribute_not_exists(branch-key-id)`
                     //#  - TableName: the configured Table Name
-                    CreateTransactWritePutItem(
+                    TransactCreateHKey(
                       input.Version,
-                      ddbTableName,
-                      BRANCH_KEY_NOT_EXIST
+                      ddbTableName
                     ),
                     //= aws-encryption-sdk-specification/framework/key-store/dynamodb-key-storage.md#writenewencryptedbranchkeyversion
                     //= type=implication
@@ -372,10 +482,10 @@ module DefaultKeyStorageInterface {
                     //#  - Item: A [record formatted item](#record-format) constructed from the active input
                     //#  - ConditionExpression: `attribute_exists(branch-key-id)`
                     //#  - TableName: the configured Table Name
-                    CreateTransactWritePutItem(
-                      input.Active,
-                      ddbTableName,
-                      BRANCH_KEY_EXISTS
+                    TransactOverwriteHKey(
+                      input.Active.Item,
+                      input.Active.Old,
+                      ddbTableName
                     )
                   ]
                 )
@@ -383,20 +493,19 @@ module DefaultKeyStorageInterface {
 
       :- Need(
         && (forall k <- input.Version.EncryptionContext.Keys :: DDB.IsValid_AttributeName(k))
-        && (forall k <- input.Active.EncryptionContext.Keys :: DDB.IsValid_AttributeName(k))
+        && (forall k <- input.Active.Item.EncryptionContext.Keys :: DDB.IsValid_AttributeName(k))
       , Types.KeyStoreException( message := ErrorMessages.ENCRYPTION_CONTEXT_EXCEEDS_DDB_LIMIT)
       );
 
       var items: DDB.TransactWriteItemList := [
-        CreateTransactWritePutItem(
+        TransactCreateHKey(
           input.Version,
-          ddbTableName,
-          BRANCH_KEY_NOT_EXIST
+          ddbTableName
         ),
-        CreateTransactWritePutItem(
-          input.Active,
-          ddbTableName,
-          BRANCH_KEY_EXISTS
+        TransactOverwriteHKey(
+          input.Active.Item,
+          input.Active.Old,
+          ddbTableName
         )
       ];
 
@@ -410,9 +519,150 @@ module DefaultKeyStorageInterface {
       var transactWriteItemsResponse? := ddbClient.TransactWriteItems(transactRequest);
       var _ :- transactWriteItemsResponse?
       .MapFailure(e => Types.ComAmazonawsDynamodb(ComAmazonawsDynamodb := e));
-
       output := Success(Types.WriteNewEncryptedBranchKeyVersionOutput);
+    }
 
+    method WriteMutationIndex'(input: Types.WriteMutationIndexInput)
+      returns (output: Result<Types.WriteMutationIndexOutput, Types.Error>)
+      requires ValidState()
+      modifies Modifies - {History}
+      decreases Modifies - {History}
+      ensures ValidState() && unchanged(History)
+      ensures WriteMutationIndexEnsuresPublicly(input, output)
+    {
+      /** Validate Input */
+      :- Need(
+        Structure.MutationCommitment?(input.MutationCommitment),
+        Types.KeyStorageException(
+          message := "Invalid mutation commitment."
+        ));
+      :- Need(
+        Structure.MutationIndex?(input.MutationIndex),
+        Types.KeyStorageException(
+          message := "Invalid mutation index."
+        ));
+      /** Construct & Issue DDB Request */
+      var ddbRequest := DDB.TransactWriteItemsInput(
+        TransactItems :=
+          [
+            TransactConditionCheckOnMutationCommitment(input.MutationCommitment, ddbTableName),
+            TransactCreateMutationIndex(input.MutationIndex, ddbTableName)
+          ]
+      );
+      var ddbResponse? := ddbClient.TransactWriteItems(ddbRequest);
+
+      /** Handle DDB Error */
+      // TODO: Wherever we write a Transaction, to explain race failure, we MUST do something like this:
+      if (ddbResponse?.Failure? && ddbResponse?.error.TransactionCanceledException?) {
+        return Failure(
+            Types.KeyStorageException(
+              message :=
+                "DDB request to Write Mutated Versions failed with DynamoDB's TransactionCanceledException. "
+                + "This MAY be caused by a race between hosts mutating the same Branch Key ID. "
+                + "The Mutation has NOT completed. "
+                + "Table Name: "+ ddbTableName
+                + "\tBranch Key ID: " + input.MutationCommitment.Identifier
+                + "\tDynamoDB Exception Message: \n" + ddbResponse?.error.Message.UnwrapOr("")));
+      }
+      var ddbResponse :- ddbResponse?
+      .MapFailure(
+        (e: DDB.Error) => wrapDdbException(
+            e:=e,
+            storageOperation:="WriteMutationIndex",
+            ddbOperation:="TransactionWriteItems",
+            identifier:=input.MutationCommitment.Identifier,
+            tableName:=ddbTableName));
+
+      return Success(Types.WriteMutationIndexOutput());
+    }
+
+
+    method {:vcs_split_on_every_assert} GetMutation' ( input: Types.GetMutationInput )
+      returns (output: Result<Types.GetMutationOutput, Types.Error>)
+      requires ValidState()
+      modifies Modifies - {History}
+      decreases Modifies - {History}
+      ensures ValidState()
+      ensures GetMutationEnsuresPublicly(input, output)
+      ensures unchanged(History)
+
+      ensures |ddbClient.History.TransactGetItems| == |old(ddbClient.History.TransactGetItems)| + 1
+      ensures output.Success?
+              ==>
+                && Seq.Last(ddbClient.History.TransactGetItems).output.Success?
+
+      ensures
+        && old(ddbClient.History.TransactGetItems) < ddbClient.History.TransactGetItems
+
+      // If the lock is invalid, must fail
+      // TODO-Mutations-FF I cannot get these prove quickly, even though they seem quite straight forward
+      // ensures
+      //   && Seq.Last(ddbClient.History.TransactGetItems).output.Success?
+      //   && Seq.Last(ddbClient.History.TransactGetItems).output.value.Responses.Some?
+      //   && |Seq.Last(ddbClient.History.TransactGetItems).output.value.Responses.value| == 2
+      //   && Seq.Last(ddbClient.History.TransactGetItems).output.value.Responses.value[0].Item.Some?
+      //   && !Structure.MutationCommitmentAttribute?(Seq.Last(ddbClient.History.TransactGetItems).output.value.Responses.value[0].Item.value)
+      //   ==> output.Failure?
+      // If the index is invalid, must fail
+      // ensures
+      //   && Seq.Last(ddbClient.History.TransactGetItems).output.Success?
+      //   && Seq.Last(ddbClient.History.TransactGetItems).output.value.Responses.Some?
+      //   && |Seq.Last(ddbClient.History.TransactGetItems).output.value.Responses.value| == 2
+      //   && Seq.Last(ddbClient.History.TransactGetItems).output.value.Responses.value[1].Item.Some?
+      //   && !Structure.MutationIndexAttribute?(Seq.Last(ddbClient.History.TransactGetItems).output.value.Responses.value[1].Item.value)
+      //   ==> output.Failure?
+    {
+      var transactItems: DDB.TransactGetItemList
+        := Seq.Map(
+        (typeStr: string)
+        =>
+          // The DDB request is a list of TransactGetItems
+          DDB.TransactGetItem(
+            Get := DDB.Get(
+              Key := DDBKeyForType(typeStr, input.Identifier),
+              TableName := ddbTableName)),
+
+        // This is the seq we are mapping over. The DDB Result will be in this order!
+        [Structure.MUTATION_COMMITMENT_TYPE, Structure.MUTATION_INDEX_TYPE]);
+
+      var ddbRequest := DDB.TransactGetItemsInput(TransactItems := transactItems);
+      var ddbResponse? := ddbClient.TransactGetItems(ddbRequest);
+
+      /** Handle DDB Error */
+      var ddbResponse :- ddbResponse?
+      .MapFailure((e: DDB.Error) =>
+                    wrapDdbException(
+                      e:=e,
+                      storageOperation:="GetMutation",
+                      ddbOperation:="TransactGetItems",
+                      identifier:=input.Identifier,
+                      tableName:=ddbTableName));
+
+        // SDKs/Smithy-Dafny/Custom Implementations of Storage MAY respond with None or an Empty Map.
+        // .NET returns an empty map, Java returns None.
+      :- Need(
+        ddbResponse.Responses.Some? && (2 == |ddbResponse.Responses.value|),
+        Types.KeyStorageException(
+          message:=
+            "GetMutation: No items returned. "
+            + "Branch Key ID: " + input.Identifier
+            + "\tTable Name: " + ddbTableName));
+
+      /** Process sensical DDB Response */
+      var lockCanidate := ddbResponse.Responses.value[0].Item;
+      var lockItem: Option<Types.MutationCommitment> :-
+        MutationCommitmentFromOptionalItem(lockCanidate, input.Identifier, ddbTableName);
+      assert lockItem.Some? ==> lockCanidate.Some? && Structure.MutationCommitmentAttribute?(lockCanidate.value);
+
+      var indexCanidate := ddbResponse.Responses.value[1].Item;
+      var indexItem: Option<Types.MutationIndex> :-
+        MutationIndexFromOptionalItem(indexCanidate, input.Identifier, ddbTableName);
+      assert indexItem.Some? ==> indexCanidate.Some? && Structure.MutationIndexAttribute?(indexCanidate.value);
+
+      return Success(
+          Types.GetMutationOutput(
+            MutationCommitment := lockItem,
+            MutationIndex := indexItem));
     }
 
     method GetEncryptedActiveBranchKey' ( input: Types.GetEncryptedActiveBranchKeyInput )
@@ -451,7 +701,8 @@ module DefaultKeyStorageInterface {
 
       ensures
         && old(ddbClient.History.GetItem) < ddbClient.History.GetItem
-        && old(ddbClient.History.TransactWriteItems) == ddbClient.History.TransactWriteItems
+      // @seebees what is this second line about? How can a GetItem have a Write in it's history
+      // && old(ddbClient.History.TransactWriteItems) == ddbClient.History.TransactWriteItems
 
       ensures
         && Seq.Last(ddbClient.History.GetItem).output.Success?
@@ -564,7 +815,6 @@ module DefaultKeyStorageInterface {
         TableName := ddbTableName
       );
 
-
       var getItemResponse? := ddbClient.GetItem(ItemRequest);
       var getItemResponse :- getItemResponse?
       .MapFailure(e => Types.ComAmazonawsDynamodb(ComAmazonawsDynamodb := e));
@@ -597,6 +847,22 @@ module DefaultKeyStorageInterface {
         Types.GetEncryptedBranchKeyVersionOutput(
           Item := versionItem
         ));
+    }
+
+    method WriteAtomicMutation'(input: Types.WriteAtomicMutationInput)
+      returns (output: Result<Types.WriteAtomicMutationOutput, Types.Error>)
+      requires ValidState()
+      modifies Modifies - {History}
+      decreases Modifies - {History}
+      ensures ValidState() && unchanged(History)
+      ensures WriteAtomicMutationEnsuresPublicly(input, output)
+
+      ensures output.Failure?
+    {
+      return Failure(
+          Types.KeyStorageException(
+            message := "At this time, WriteAtomicMutation is not supported."
+          ));
     }
 
     method GetEncryptedBeaconKey' ( input: Types.GetEncryptedBeaconKeyInput )
@@ -708,12 +974,467 @@ module DefaultKeyStorageInterface {
             LogicalName := logicalKeyStoreNameUtf8
           ));
     }
+
+    function method DDBKeyForType(
+      typeStr: string,
+      identifier: string
+    ): (key: DDB.Key)
+    {
+      map[
+        Structure.BRANCH_KEY_IDENTIFIER_FIELD := DDB.AttributeValue.S(identifier),
+        Structure.TYPE_FIELD := DDB.AttributeValue.S(typeStr)
+      ]
+    }
+
+    // This a TransactGetItems for 5 items
+    method GetItemsForInitializeMutation' ( input: Types.GetItemsForInitializeMutationInput )
+      returns (output: Result<Types.GetItemsForInitializeMutationOutput, Types.Error>)
+      requires  ValidState()
+      modifies Modifies - {History}
+      // Dafny will skip type parameters when generating a default decreases clause.
+      decreases Modifies - {History}
+      ensures ValidState()
+      ensures GetItemsForInitializeMutationEnsuresPublicly(input, output)
+      ensures unchanged(History)
+    {
+      /** Construct & Issue DDB Request */
+      var transactItems: DDB.TransactGetItemList
+        := Seq.Map(
+        (typeStr: string)
+        =>
+          // The DDB request is a list of TransactGetItems
+          DDB.TransactGetItem(
+            Get := DDB.Get(
+              Key := DDBKeyForType(typeStr, input.Identifier),
+              TableName := ddbTableName)),
+
+        // This is the seq we are mapping over. The DDB Result will be in this order!
+        [Structure.MUTATION_COMMITMENT_TYPE, Structure.BRANCH_KEY_ACTIVE_TYPE,
+         Structure.BEACON_KEY_TYPE_VALUE, Structure.MUTATION_INDEX_TYPE]);
+
+      var ddbRequest := DDB.TransactGetItemsInput(TransactItems := transactItems);
+      var ddbResponse? := ddbClient.TransactGetItems(ddbRequest);
+
+      /** Handle DDB Error */
+      var ddbResponse :- ddbResponse?
+      .MapFailure((e: DDB.Error) =>
+                    wrapDdbException(
+                      e:=e,
+                      storageOperation:="GetItemsForInitializeMutation",
+                      ddbOperation:="TransactGetItems",
+                      identifier:=input.Identifier,
+                      tableName:=ddbTableName));
+
+        // SDKs/Smithy-Dafny/Custom Implementations of Storage MAY respond with None or an Empty Map.
+        // .NET returns an empty map, Java returns None.
+      :- Need(
+        ddbResponse.Responses.Some? && (4 == |ddbResponse.Responses.value|),
+        Types.KeyStorageException(
+          message:=
+            "GetItemsForInitializeMutation: No items returned. "
+            + "Branch Key ID: " + input.Identifier
+            + "\tTable Name: " + ddbTableName));
+
+      /** Process sensical DDB Response */
+      var lockItem: Option<Types.MutationCommitment> :-
+        MutationCommitmentFromOptionalItem(ddbResponse.Responses.value[0].Item, input.Identifier, ddbTableName);
+
+      :- Need(
+        ddbResponse.Responses.value[1].Item.Some? && (0 < |ddbResponse.Responses.value[1].Item.value|),
+        Types.KeyStorageException(
+          message:=
+            "GetItemsForInitializeMutation: Could not find the ACTIVE Item. "
+            + "Branch Key ID: " + input.Identifier
+            + "\tTable Name: " + ddbTableName));
+      var activeItem: Types.EncryptedHierarchicalKey :-
+        EncryptedHierarchicalKeyFromItem(
+          ddbResponse.Responses.value[1].Item.value, logicalKeyStoreName, input.Identifier, ddbTableName);
+
+      :- Need(
+        ddbResponse.Responses.value[2].Item.Some?  && (0 < |ddbResponse.Responses.value[2].Item.value|),
+        Types.KeyStorageException(
+          message:=
+            "GetItemsForInitializeMutation: Could not find the Beacon Item. "
+            + "Branch Key ID: " + input.Identifier
+            + "\tTable Name: " + ddbTableName));
+      var beaconItem: Types.EncryptedHierarchicalKey :-
+        EncryptedHierarchicalKeyFromItem(
+          ddbResponse.Responses.value[2].Item.value, logicalKeyStoreName, input.Identifier, ddbTableName);
+
+      var indexItem: Option<Types.MutationIndex> :-
+        MutationIndexFromOptionalItem(ddbResponse.Responses.value[3].Item, input.Identifier, ddbTableName);
+
+        /** Validate DDB Responses */
+      :- Need(
+        && Structure.ActiveHierarchicalSymmetricKey?(activeItem),
+        Types.KeyStorageException(
+          message:=
+            "Item returned for the ACTIVE is malformed. TableName: " + ddbTableName + "\tBranch Key ID: " + input.Identifier
+        ));
+
+      :- Need(
+        && Structure.ActiveHierarchicalSymmetricBeaconKey?(beaconItem),
+        Types.KeyStorageException(
+          message:=
+            "Item returned for Beacon Key is malformed. TableName: " + ddbTableName + "\tBranch Key ID: " + input.Identifier
+        ));
+
+      return Success(
+          Types.GetItemsForInitializeMutationOutput(
+            ActiveItem := activeItem,
+            BeaconItem := beaconItem,
+            MutationCommitment := lockItem,
+            MutationIndex := indexItem
+          ));
+    }
+
+    /** A transaction write for 5 items, conditioned on No Mutation Lock Or Index exsisting for Identifier.*/
+    /** One of the items is a new Active; it is conditioned on the oldActive's enc still being present at write time.*/
+    method WriteInitializeMutation' ( input: Types.WriteInitializeMutationInput )
+      returns (output: Result<Types.WriteInitializeMutationOutput, Types.Error>)
+      requires ValidState()
+      modifies Modifies - {History}
+      decreases Modifies - {History}
+      ensures ValidState() && unchanged(History)
+      ensures WriteInitializeMutationEnsuresPublicly(input, output)
+
+    {
+      :- Need(
+        Structure.MutationCommitment?(input.MutationCommitment),
+        Types.KeyStorageException(
+          message := "Invalid mutation commitment."
+        ));
+      :- Need(
+        Structure.MutationIndex?(input.MutationIndex),
+        Types.KeyStorageException(
+          message := "Invalid mutation index."
+        ));
+
+      if (input.Version.mutate?) {
+        return Failure(
+            Types.KeyStorageException(
+              message := "At this time, only rotation is supported."
+            ));
+      }
+
+      :- Need(
+        && (forall k <- input.Version.rotate.EncryptionContext.Keys :: DDB.IsValid_AttributeName(k))
+        && (forall k <- input.Active.Item.EncryptionContext.Keys :: DDB.IsValid_AttributeName(k)),
+        Types.KeyStorageException( message := ErrorMessages.ENCRYPTION_CONTEXT_EXCEEDS_DDB_LIMIT)
+      );
+
+        /** Validate Inputs can be mapped to DDB Items */
+      :- Need(
+        && (forall k <- input.Beacon.Item.EncryptionContext.Keys :: DDB.IsValid_AttributeName(k)),
+        Types.KeyStorageException( message := ErrorMessages.ENCRYPTION_CONTEXT_EXCEEDS_DDB_LIMIT)
+      );
+
+      /** Convert Inputs to DDB Items.*/
+      var items: DDB.TransactWriteItemList := [
+        TransactCreateHKey(
+          input.Version.rotate,
+          ddbTableName
+        ),
+        TransactOverwriteHKey(
+          input.Active.Item,
+          input.Active.Old,
+          ddbTableName
+        ),
+        TransactOverwriteHKey(
+          input.Beacon.Item,
+          input.Beacon.Old,
+          ddbTableName
+        ),
+        TransactCreateMutationCommitment(
+          input.MutationCommitment,
+          ddbTableName
+        ),
+        TransactCreateMutationIndex(
+          input.MutationIndex,
+          ddbTableName)
+      ];
+      var transactRequest := DDB.TransactWriteItemsInput(
+        TransactItems := items
+      );
+
+      var transactWriteItemsResponse? := ddbClient.TransactWriteItems(transactRequest);
+      // TODO-Mutations-FF: we need to check the cancellation reason for
+      // ConditionalCheckFailed on the Active item (VersionRaceException)
+      // OR the Mutation Lock (MutationCommitmentException)
+      // OR something else.
+      var _ :- transactWriteItemsResponse?
+      .MapFailure(e => wrapDdbException(
+                      e:=e,
+                      storageOperation:="WriteInitializeMutation",
+                      ddbOperation:="TransactWriteItems",
+                      identifier:=input.Active.Item.Identifier,
+                      tableName:=ddbTableName));
+      // This is a Smithy Modeled Operation; the output MUST be a Structure
+      output := Success(Types.WriteInitializeMutationOutput());
+    }
+
+    static const queryForVersionsKeyExpression: DDB.KeyExpression := "#pk = :pk AND begins_with( #sk, :decryptOnlyPrefix )"
+
+    method QueryForVersions' ( input: Types.QueryForVersionsInput )
+      returns (output: Result<Types.QueryForVersionsOutput, Types.Error>)
+      requires ValidState()
+      modifies Modifies - {History}
+      decreases Modifies - {History}
+      ensures ValidState() && unchanged(History)
+      ensures QueryForVersionsEnsuresPublicly(input, output)
+    {
+      /** Construct & Issue DDB Request */
+      var exclusiveStartKey: Option<DDB.Key> := None;
+      if (input.ExclusiveStartKey.Some?) {
+        var decodedLastKey :- BlobToExclusiveStartKey(
+          input.ExclusiveStartKey.value,
+          input.Identifier);
+        exclusiveStartKey := Some(decodedLastKey);
+      }
+      :- Need(0 < input.PageSize,
+              Types.KeyStorageException(message:="DynamoDB Encrypted Key Storage will not Query for page size of 0."));
+      var exprAttributeValues: DDB.ExpressionAttributeValueMap := map[
+        ":pk" := DDB.AttributeValue.S(input.Identifier),
+        ":decryptOnlyPrefix" := DDB.AttributeValue.S("branch:version:")];
+      var ddbRequest := DDB.QueryInput(
+        TableName := ddbTableName,
+        Limit := Some(input.PageSize),
+        ConsistentRead := Some(true),
+        ExclusiveStartKey := exclusiveStartKey,
+        KeyConditionExpression := Some(queryForVersionsKeyExpression),
+        ExpressionAttributeNames := Some(INDEX_EXP_ATT_NAMES),
+        ExpressionAttributeValues := Some(exprAttributeValues)
+      );
+      var ddbResponse? := ddbClient.Query(ddbRequest);
+
+      /** Handle DDB Error */
+      var ddbResponse :- ddbResponse?
+      .MapFailure(
+        (e: DDB.Error) => wrapDdbException(
+            e:=e,
+            storageOperation:="QueryForVersions",
+            ddbOperation:="Query",
+            identifier:=input.Identifier,
+            tableName:=ddbTableName));
+
+      /** Process sensical DDB Response */
+      var lastKeyBlob: seq<Types.UInt.uint8> := [];
+      var lastKeyEmpty: bool :=
+        // It is not clear if SDKs/Smithy-Dafny/Custom Implementations of Storage will respond with None or an Empty Map.
+        ddbResponse.LastEvaluatedKey.None? || (ddbResponse.LastEvaluatedKey.Some? && |ddbResponse.LastEvaluatedKey.value| == 0);
+
+      if (!lastKeyEmpty) {
+        lastKeyBlob :- LastEvaluatedKeyToBlob(ddbResponse.LastEvaluatedKey.value);
+      }
+      if (ddbResponse.Items.None? || ( |ddbResponse.Items.value| == 0) ) {
+        return Success(Types.QueryForVersionsOutput(
+                         ExclusiveStartKey := lastKeyBlob,
+                         Items := []
+                       ));
+      }
+
+      /* Map DDB items to Branch Keys.*/
+      var branchKeys: seq<Types.EncryptedHierarchicalKey> :- Seq.MapWithResult(
+        // Dafny requires the type of the element being mapped over, or it feaks out.
+        (item: DDB.AttributeMap)
+        =>
+          /* Convert DDB Item to Branch Key. */
+          var branchKey :- EncryptedHierarchicalKeyFromItem(item, logicalKeyStoreName, input.Identifier, ddbTableName);
+          /* Validate that Branch Key is a Version, or Decrypt Only, Branch Key Type. */
+          :- Need(
+               branchKey.Type.HierarchicalSymmetricVersion?,
+               Types.KeyStorageException(
+                 message:="Unexpected item returned by DDB. TableName: " + ddbTableName + "\tBranch Key ID: " + input.Identifier
+               ));
+          Success(branchKey),
+        ddbResponse.Items.value
+      );
+
+      return Success(
+          Types.QueryForVersionsOutput(
+            ExclusiveStartKey := lastKeyBlob,
+            Items := branchKeys
+          ));
+    }
+
+    /** Transaction OverWrite up to 98 Decryt Only Items,
+       with a Global Condition on the M-Commitment.
+       The Mutation Index is also updated via an Optimistic Lock.
+       If the mutation is complete, the M-Commitment & M-Index are deleted.
+     */
+    method WriteMutatedVersions' ( input: Types.WriteMutatedVersionsInput )
+      returns (output: Result<Types.WriteMutatedVersionsOutput, Types.Error>)
+      requires && ValidState()
+      modifies Modifies - {History}
+      decreases Modifies - {History}
+      ensures unchanged(History) && ValidState()
+      ensures WriteMutatedVersionsEnsuresPublicly(input, output)
+    {
+      /** Validate Input */
+      :- Need(
+        |input.Items| < DDB_MAX_MUTATION_WRITE_PAGE_SIZE,
+        Types.KeyStorageException(message:="DynamoDB Encrypted Key Storage can only write page sizes less than " + DDB_MAX_MUTATION_WRITE_PAGE_SIZE_str + "."
+        ));
+      :- Need(
+        0 < |input.MutationCommitment.Original|,
+        Types.KeyStorageException(message:="Original State MUST NOT be empty."
+        ));
+      :- Need(
+        0 < |input.MutationCommitment.Terminal|,
+        Types.KeyStorageException(message:="Terminal State MUST NOT be empty."
+        ));
+      :- Need(
+        Structure.MutationIndex?(input.MutationIndex.Index),
+        Types.KeyStorageException(message:="Mutation Index MUST be valid."
+        ));
+
+      /** Convert Items to DDB */
+      var items: seq<DDB.TransactWriteItem> :- Seq.MapWithResult(
+        (branchKey: Types.OverWriteEncryptedHierarchicalKey)
+        =>
+          /* All Attribute Names MUST comply with DDB's limits.*/
+          /* Attribute Names are the "keys" of the Encryption Context.*/
+          :- Need(
+               && (forall k <- branchKey.Item.EncryptionContext.Keys :: DDB.IsValid_AttributeName(k)),
+               Types.KeyStorageException( message := ErrorMessages.ENCRYPTION_CONTEXT_EXCEEDS_DDB_LIMIT)
+             );
+          /* Only Version, or Decrypt Only, items are permitted.*/
+          :- Need(
+               branchKey.Item.Type.HierarchicalSymmetricVersion?,
+               Types.KeyStorageException(
+                 message :=
+                   "WriteMutatedVersions of DynamoDB Encrypted Key Storage ONLY writes Decrypt Only Items to Storage. "
+                   + "Encountered a non-Decrypt Only Item."
+               ));
+          /* The branch key is valid for DDB; create a Put request.*/
+          var overWrite := TransactOverwriteHKey(
+                             branchKey.Item,
+                             branchKey.Old,
+                             ddbTableName);
+          Success(overWrite),
+        input.Items);
+
+      var mLock := input.MutationCommitment;
+      var mLockAction := if input.EndMutation
+      then TransactConditionalDeleteMutationCommitment(mLock, ddbTableName)
+      else TransactConditionCheckOnMutationCommitment(mLock, ddbTableName);
+      var mIndex := input.MutationIndex;
+      var mIndexAction :=
+        if input.EndMutation
+        then TransactConditionalDeleteMutationIndex(mIndex.Index, mIndex.Old, ddbTableName)
+        else TransactOverwriteMutationIndex(mIndex.Index, mIndex.Old, ddbTableName);
+      /** Construct & Issue DDB Request */
+      var ddbRequest := DDB.TransactWriteItemsInput(
+        TransactItems := [mLockAction,  mIndexAction] + items
+      );
+      var ddbResponse? := ddbClient.TransactWriteItems(ddbRequest);
+
+      /** Handle DDB Error */
+      // TODO: Wherever we write a Transaction, to explain race failure, we MUST do something like this:
+      if (ddbResponse?.Failure? && ddbResponse?.error.TransactionCanceledException?) {
+        return Failure(
+            Types.KeyStorageException(
+              message :=
+                "DDB request to Write Mutated Versions was failed by DDB with TransactionCanceledException. "
+                + "This MAY be caused by a race between hosts mutating the same Branch Key ID. "
+                + "The Mutation has NOT completed. "
+                + "Table Name: "+ ddbTableName
+                + "\tBranch Key ID: " + mLock.Identifier
+                + "\tDDB Exception Message: \n" + ddbResponse?.error.Message.UnwrapOr("")));
+      }
+      var ddbResponse :- ddbResponse?
+      .MapFailure(
+        (e: DDB.Error) => wrapDdbException(
+            e:=e,
+            storageOperation:="WriteMutatedVersions",
+            ddbOperation:="TransactionWriteItems",
+            identifier:=mLock.Identifier,
+            tableName:=ddbTableName));
+
+      return Success(Types.WriteMutatedVersionsOutput());
+    }
+
+    method DeleteMutation' ( input: Types.DeleteMutationInput )
+      returns (output: Result<Types.DeleteMutationOutput, Types.Error>)
+      requires ValidState()
+      modifies Modifies - {History}
+      decreases Modifies - {History}
+      ensures ValidState() && unchanged(History)
+      ensures DeleteMutationEnsuresPublicly(input, output)
+
+      ensures !Structure.MutationCommitment?(input.MutationCommitment) ==> output.Failure?
+      ensures
+        && Structure.MutationCommitment?(input.MutationCommitment) ==>(
+            && |ddbClient.History.TransactWriteItems| == |old(ddbClient.History.TransactWriteItems)| + 1
+            && old(ddbClient.History.TransactWriteItems) < ddbClient.History.TransactWriteItems
+            && (output.Success? ==> Seq.Last(ddbClient.History.TransactWriteItems).output.Success?)
+            && (Seq.Last(ddbClient.History.TransactWriteItems).output.Failure? ==> output.Failure?))
+
+      ensures
+        output.Success?
+        ==>
+          && Seq.Last(ddbClient.History.TransactWriteItems).input
+             == DDB.TransactWriteItemsInput(
+                  TransactItems := [
+                    TransactConditionalDeleteMutationCommitment(
+                      input.MutationCommitment,
+                      ddbTableName),
+                    TransactNoConditionDeleteMutationIndex(
+                      input.MutationCommitment.Identifier,
+                      ddbTableName
+                    )
+                  ]
+                )
+    {
+      /** Validate Input */
+      :- Need(
+        Structure.MutationCommitment?(input.MutationCommitment),
+        Types.KeyStorageException(message:="Mutation Index must be valid."));
+
+      var items: DDB.TransactWriteItemList := [
+        TransactConditionalDeleteMutationCommitment(
+          input.MutationCommitment,
+          ddbTableName),
+        TransactNoConditionDeleteMutationIndex(
+          input.MutationCommitment.Identifier,
+          ddbTableName
+        )
+      ];
+
+      /** Construct & Issue DDB Request */
+      var ddbRequest := DDB.TransactWriteItemsInput(
+        TransactItems := items
+      );
+      var ddbResponse? := ddbClient.TransactWriteItems(ddbRequest);
+
+      /** Handle DDB Error */
+      // TODO: Wherever we write a Transaction, to explain race failure, we MUST do something like this:
+      if (ddbResponse?.Failure? && ddbResponse?.error.TransactionCanceledException?) {
+        return Failure(
+            Types.KeyStorageException(
+              message :=
+                "DDB request to Delete Mutation Lock & Index was failed by DDB with TransactionCanceledException. "
+                + "This MAY be caused by a race between hosts mutating the same Branch Key ID. "
+                + "The Mutation has NOT completed. "
+                + "Table Name: "+ ddbTableName
+                + "\tBranch Key ID: " + input.MutationCommitment.Identifier
+                + "\tDDB Exception Message: \n" + ddbResponse?.error.Message.UnwrapOr("")));
+      }
+      var ddbResponse :- ddbResponse?
+      .MapFailure(
+        (e: DDB.Error) => wrapDdbException(
+            e:=e,
+            storageOperation:="DeleteMutation",
+            ddbOperation:="TransactionWriteItems",
+            identifier:=input.MutationCommitment.Identifier,
+            tableName:=ddbTableName));
+      return Success(Types.DeleteMutationOutput());
+    }
   }
 
-  function method CreateTransactWritePutItem(
+  function method TransactCreateHKey(
     encryptedKey: Types.EncryptedHierarchicalKey,
-    tableName: DDB.TableName,
-    ConditionExpression: ConditionExpression
+    tableName: DDB.TableName
   ): (output: DDB.TransactWriteItem)
     requires (forall k <- encryptedKey.EncryptionContext.Keys :: DDB.IsValid_AttributeName(k))
   {
@@ -722,12 +1443,272 @@ module DefaultKeyStorageInterface {
         DDB.Put(
           Item := ToAttributeMap(encryptedKey),
           TableName := tableName,
-          ConditionExpression := Some(
-            match ConditionExpression
-            case BRANCH_KEY_NOT_EXIST() => BRANCH_KEY_NOT_EXIST_CONDITION
-            case BRANCH_KEY_EXISTS() => BRANCH_KEY_EXISTS_CONDITION
-          ),
+          ConditionExpression := Some(BRANCH_KEY_NOT_EXIST_CONDITION),
           ExpressionAttributeNames := Some(BRANCH_KEY_EXISTS_EXPRESSION_ATTRIBUTE_NAMES)))
     )
+  }
+
+  function method TransactCreateMutationCommitment(
+    mutationLock: Types.MutationCommitment,
+    tableName: DDB.TableName
+  ): (output: DDB.TransactWriteItem)
+    requires Structure.MutationCommitment?(mutationLock)
+  {
+    DDB.TransactWriteItem(
+      Put := Some(
+        DDB.Put(
+          Item := Structure.MutationCommitmentToAttributeMap(mutationLock),
+          TableName := tableName,
+          ConditionExpression := Some(BRANCH_KEY_NOT_EXIST_CONDITION),
+          ExpressionAttributeNames := Some(BRANCH_KEY_EXISTS_EXPRESSION_ATTRIBUTE_NAMES)))
+    )
+  }
+
+  function method TransactCreateMutationIndex(
+    mutationIndex: Types.MutationIndex,
+    tableName: DDB.TableName
+  ): (output: DDB.TransactWriteItem)
+    requires Structure.MutationIndex?(mutationIndex)
+  {
+    DDB.TransactWriteItem(
+      Put := Some(
+        DDB.Put(
+          Item := Structure.MutationIndexToAttributeMap(mutationIndex),
+          TableName := tableName,
+          ConditionExpression := Some(BRANCH_KEY_NOT_EXIST_CONDITION),
+          ExpressionAttributeNames := Some(BRANCH_KEY_EXISTS_EXPRESSION_ATTRIBUTE_NAMES)))
+    )
+  }
+
+  function method TransactConditionalDeleteMutationCommitment(
+    mLock: Types.MutationCommitment,
+    tableName: DDB.TableName
+  ): (output: DDB.TransactWriteItem)
+  {
+    var check := checkForMutationCommitment(mLock);
+    DDB.TransactWriteItem(
+      Delete := Some(
+        DDB.Delete(
+          Key :=
+            map[
+              Structure.BRANCH_KEY_IDENTIFIER_FIELD := DDB.AttributeValue.S(mLock.Identifier),
+              Structure.TYPE_FIELD := DDB.AttributeValue.S(Structure.MUTATION_COMMITMENT_TYPE)
+            ],
+          TableName := tableName,
+          ConditionExpression := Some(check.ConditionExpression),
+          ExpressionAttributeNames := Some(check.ExpressionAttributeNames),
+          ExpressionAttributeValues := Some(check.ExpressionAttributeValues)
+        )))
+  }
+
+  function method TransactOverwriteHKey(
+    item: Types.EncryptedHierarchicalKey,
+    oldItem: Types.EncryptedHierarchicalKey,
+    tableName: DDB.TableName
+  ): (output: DDB.TransactWriteItem)
+    requires (forall k <- item.EncryptionContext.Keys :: DDB.IsValid_AttributeName(k))
+  {
+    var check := checkForOldEnc(oldItem.CiphertextBlob);
+    DDB.TransactWriteItem(
+      Put := Some(
+        DDB.Put(
+          Item := ToAttributeMap(item),
+          TableName := tableName,
+          ConditionExpression := Some(check.ConditionExpression),
+          ExpressionAttributeNames := Some(check.ExpressionAttributeNames),
+          ExpressionAttributeValues := Some(check.ExpressionAttributeValues)
+        )))
+  }
+
+  function method TransactOverwriteMutationIndex(
+    index: Types.MutationIndex,
+    oldIndex: Types.MutationIndex,
+    tableName: DDB.TableName
+  ): (output: DDB.TransactWriteItem)
+    requires Structure.MutationIndex?(index)
+  {
+    var check := ConditionForMutationIndex(oldIndex);
+    DDB.TransactWriteItem(
+      Put := Some(
+        DDB.Put(
+          Item := Structure.MutationIndexToAttributeMap(index),
+          TableName := tableName,
+          ConditionExpression := Some(check.ConditionExpression),
+          ExpressionAttributeNames := Some(check.ExpressionAttributeNames),
+          ExpressionAttributeValues := Some(check.ExpressionAttributeValues)
+        )))
+  }
+
+  function method TransactConditionalDeleteMutationIndex(
+    index: Types.MutationIndex,
+    oldIndex: Types.MutationIndex,
+    tableName: DDB.TableName
+  ): (output: DDB.TransactWriteItem)
+    requires Structure.MutationIndex?(index)
+  {
+    var check := ConditionForMutationIndex(oldIndex);
+    DDB.TransactWriteItem(
+      Delete := Some(
+        DDB.Delete(
+          Key :=
+            map[
+              Structure.BRANCH_KEY_IDENTIFIER_FIELD := DDB.AttributeValue.S(index.Identifier),
+              Structure.TYPE_FIELD := DDB.AttributeValue.S(Structure.MUTATION_INDEX_TYPE)
+            ],
+          TableName := tableName,
+          ConditionExpression := Some(check.ConditionExpression),
+          ExpressionAttributeNames := Some(check.ExpressionAttributeNames),
+          ExpressionAttributeValues := Some(check.ExpressionAttributeValues)
+        )))
+  }
+
+  function method TransactNoConditionDeleteMutationIndex(
+    identifier: string,
+    tableName: DDB.TableName
+  ): (output: DDB.TransactWriteItem)
+  {
+    DDB.TransactWriteItem(
+      Delete := Some(
+        DDB.Delete(
+          Key :=
+            map[
+              Structure.BRANCH_KEY_IDENTIFIER_FIELD := DDB.AttributeValue.S(identifier),
+              Structure.TYPE_FIELD := DDB.AttributeValue.S(Structure.MUTATION_INDEX_TYPE)
+            ],
+          TableName := tableName
+        )))
+  }
+
+  datatype check = | check(
+    nameonly ConditionExpression: DDB.ConditionExpression ,
+    nameonly ExpressionAttributeNames: DDB.ExpressionAttributeNameMap ,
+    nameonly ExpressionAttributeValues: DDB.ExpressionAttributeValueMap)
+
+  /** Assert the cipherText of the Active Item has not changed since it was read.*/
+  function method checkForOldEnc(
+    oldCiphertextBlob: seq<Types.UInt.uint8>
+  ): (output: check)
+  {
+    check(
+      ConditionExpression := "attribute_exists(#pk) AND " + Structure.ENC_FIELD + " = :encOld",
+      ExpressionAttributeNames := map["#pk" := Structure.BRANCH_KEY_IDENTIFIER_FIELD],
+      ExpressionAttributeValues := map[":encOld" := DDB.AttributeValue.B(oldCiphertextBlob)])
+  }
+
+  function method checkForMutationCommitment(
+    mLock: Types.MutationCommitment
+  ): (output: check)
+  {
+    check(
+      ConditionExpression :=
+        "attribute_exists(#pk)"
+        + " AND original = :original"
+        + " AND terminal = :terminal"
+        + " AND " + Structure.ENC_FIELD + " = :encOld"
+        + " AND #uuid = :" + Structure.M_UUID,
+      ExpressionAttributeNames := map[
+        "#pk" := Structure.BRANCH_KEY_IDENTIFIER_FIELD, // "#pk":="branch-key-id"
+        "#uuid" := Structure.M_UUID // "#uuid" := "uuid"
+      ],
+      ExpressionAttributeValues :=
+        map[
+          ":original" := DDB.AttributeValue.B(mLock.Original),
+          ":terminal" := DDB.AttributeValue.B(mLock.Terminal),
+          ":encOld" := DDB.AttributeValue.B(mLock.CiphertextBlob),
+          ":" + Structure.M_UUID := DDB.AttributeValue.S(mLock.UUID)
+        ]
+    )
+  }
+
+  /** Assert a Mutation Lock exists for Branch Key ID, with Original and Terminal as expected.*/
+  /** For use with WriteMutatedVersions. */
+  function method TransactConditionCheckOnMutationCommitment(
+    mLock: Types.MutationCommitment,
+    tableName: DDB.TableName
+  ): (output: DDB.TransactWriteItem)
+  {
+    var check := checkForMutationCommitment(mLock);
+    var conditionCheck
+      :=
+      DDB.ConditionCheck(
+        Key := map[
+          Structure.BRANCH_KEY_IDENTIFIER_FIELD := DDB.AttributeValue.S(mLock.Identifier),
+          Structure.TYPE_FIELD := DDB.AttributeValue.S(Structure.MUTATION_COMMITMENT_TYPE)
+        ],
+        TableName := tableName,
+        ConditionExpression := check.ConditionExpression,
+        ExpressionAttributeNames := Some(check.ExpressionAttributeNames),
+        ExpressionAttributeValues := Some(check.ExpressionAttributeValues)
+      );
+    DDB.TransactWriteItem(ConditionCheck := Some(conditionCheck))
+  }
+
+  function method ConditionForMutationIndex(
+    oldIndex: Types.MutationIndex
+  ): (output: check)
+  {
+    check(
+      ConditionExpression :=
+        "attribute_exists(#pk)"
+        + " AND " + Structure.M_PAGE_INDEX + " = :" + Structure.M_PAGE_INDEX + "Old"
+        + " AND " + Structure.ENC_FIELD + " = :" + Structure.ENC_FIELD + "Old"
+        + " AND #uuid = :" + Structure.M_UUID,
+      ExpressionAttributeNames := map[
+        "#pk" := Structure.BRANCH_KEY_IDENTIFIER_FIELD, // "#pk":="branch-key-id"
+        "#uuid" := Structure.M_UUID // "#uuid" := "uuid"
+      ],
+      ExpressionAttributeValues :=
+        map[
+          ":" + Structure.M_PAGE_INDEX + "Old" := DDB.AttributeValue.B(oldIndex.PageIndex),
+          ":" + Structure.ENC_FIELD + "Old" := DDB.AttributeValue.B(oldIndex.CiphertextBlob),
+          ":" + Structure.M_UUID := DDB.AttributeValue.S(oldIndex.UUID)
+        ]
+    )
+  }
+
+  /** It is a BREAKING CHANGE to use this for Key Store Operations released in MPL v1.0.2. */
+  function method wrapDdbException(
+    nameonly e: DDB.Error,
+    nameonly storageOperation: string,
+    nameonly ddbOperation: string,
+    nameonly identifier: string,
+    nameonly tableName: string
+  ): (storageException: Types.Error)
+  {
+    // TODO Benerate KeyStorageException to have a message field and an Error field
+    // that can hold either Opaque or DDB Error
+    match e {
+      case Opaque(obj) => Types.Opaque(obj) //https://github.com/smithy-lang/smithy-dafny/issues/450#issuecomment-2322149920
+      case IdempotentParameterMismatchException(Message) => Types.KeyStorageException(
+        message :=
+          "DDB through an exception for " +  storageOperation + "'s " + ddbOperation + ". Table Name: "
+          + tableName
+          + "\tBranch Key ID: " + identifier
+          + "\tDDB Message: " + Message.UnwrapOr(""))
+      case InvalidEndpointException(Message) => Types.KeyStorageException(
+        message :=
+          "DDB through an exception for " +  storageOperation + "'s " + ddbOperation + ". Table Name: "
+          + tableName
+          + "\tBranch Key ID: " + identifier
+          + "\tDDB Message: " + Message.UnwrapOr(""))
+      case TransactionInProgressException(Message) => Types.KeyStorageException(
+        message :=
+          "DDB through an exception for " +  storageOperation + "'s " + ddbOperation + ". Table Name: "
+          + tableName
+          + "\tBranch Key ID: " + identifier
+          + "\tDDB Message: " + Message.UnwrapOr(""))
+      case TransactionCanceledException(Message, _) => Types.KeyStorageException(
+        message :=
+          "DDB through an exception for " +  storageOperation + "'s " + ddbOperation + ". Table Name: "
+          + tableName
+          + "\tBranch Key ID: " + identifier
+          + "\tDDB Message: " + Message.UnwrapOr(""))
+      case _ => Types.KeyStorageException(
+        message :=
+          "DDB through an exception for " +  storageOperation + "'s " + ddbOperation + ". Table Name: "
+          + tableName
+          + "\tBranch Key ID: " + identifier
+          + "\tDDB Message: " + e.message.UnwrapOr(""))
+    }
   }
 }
